VCVio/CryptoFoundations/SignatureAlg.lean
@@ -1,0 +1,68 @@
+/-
+Copyright (c) 2024 Devon Tuma. All rights reserved.
+Released under Apache 2.0 license as described in the file LICENSE.
+Authors: Devon Tuma
+-/
+import VCVio.CryptoFoundations.SecExp
+import VCVio.OracleComp.Constructions.UniformSelect
+import VCVio.OracleComp.OracleSpec.Append
+import VCVio.OracleComp.SimSemantics.QueryTracking.LoggingOracle
+
+import VCVio.OracleComp.SimSemantics.QueryTracking.CachingOracle
+import VCVio.OracleComp.SimSemantics.Append
+
+/-!
+# Asymmetric Encryption Schemes.
+
+This file defines a type `AsymmEncAlg spec M PK SK C` to represent an protocol
+for asymmetric encryption using oracles in `spec`, with message space `M`,
+public/secret keys `PK` and `SK`, and ciphertext space `C`.
+-/
+
+open OracleSpec OracleComp
+
+structure SignatureAlg (spec : OracleSpec)
+    (M PK SK S : Type) extends OracleAlg spec where
+  keygen : Unit → OracleComp spec (PK × SK)
+  sign : PK → SK → M → OracleComp spec S
+  verify : PK → M → S → OracleComp spec Bool
+
+
+namespace SignatureAlg
+
+variable {spec : OracleSpec}
+    {M PK SK S : Type} [Inhabited S] [DecidableEq M] [DecidableEq S]
+    [Fintype S]
+
+def soundnessExp (sigAlg : SignatureAlg spec M PK SK S)
+    (m : M) : SecExp spec (PK × SK) where
+  inpGen := sigAlg.keygen ()
+  main := λ (pk, sk) ↦ do
+    let σ ← sigAlg.sign pk sk m
+    sigAlg.verify pk m σ
+  __ := sigAlg
+
+def unforgeableAdv (_sigAlg : SignatureAlg spec M PK SK S) :=
+SecAdv (spec ++ (M →ₒ S)) PK (M × S)
+
+def signingOracle (sigAlg : SignatureAlg spec M PK SK S)
+    (pk : PK) (sk : SK) :
+    (M →ₒ S) →[QueryLog (M →ₒ S)]ₛₒ spec :=
+  λ () m log ↦ do
+    let σ ← sigAlg.sign pk sk m
+    return (σ, log.logQuery m σ)
+
+def unforgeableExp {sigAlg : SignatureAlg spec M PK SK S}
+    (adv : SecAdv (spec ++ (M →ₒ S)) PK (M × S)) :
+    SecExp spec (PK × SK) where
+  inpGen := sigAlg.keygen ()
+  main := λ ⟨pk, sk⟩ ↦ do
+    let ((m, σ), ((), log)) ←
+      simulate (idOracle ++ₛₒ sigAlg.signingOracle pk sk)
+        (adv.run pk) ((), λ _ ↦ [])
+    let b ← sigAlg.verify pk m σ
+    return (b && !(log.wasQueried () m))
+  __ := sigAlg
+
+
+end SignatureAlg
