VCVio/OracleComp/SimSemantics/QueryTracking/CachingOracle.lean
@@ -4,11 +4,14 @@ Released under Apache 2.0 license as described in the file LICENSE.
 Authors: Devon Tuma
 -/
 import VCVio.OracleComp.SimSemantics.Simulate
+import VCVio.OracleComp.Constructions.UniformSelect
 
 /-!
 # Caching Queries Made by a Computation
 
 -/
+
+open Option
 
 namespace OracleSpec
 
@@ -19,14 +22,22 @@ def QueryCache.cacheQuery {spec : OracleSpec} (cache : QueryCache spec) {i : spe
     (t : spec.domain i) (u : spec.range i) : QueryCache spec :=
   Function.update cache i (Function.update (cache i) t u)
 
+instance : EmptyCollection (QueryCache spec) := ⟨λ _ _ ↦ none⟩
+
 end OracleSpec
 
 open OracleComp OracleSpec
 
 def cachingOracle {spec : OracleSpec} :
     spec →[QueryCache spec]ₛₒ spec :=
-  λ i ⟨t, cache⟩ ↦ match cache i t with
+  λ i t cache ↦ match cache i t with
     | Option.some u => return (u, cache)
     | Option.none => do
         let u ← query i t
         return (u, cache.cacheQuery t u)
+
+def randOracle {spec : OracleSpec}
+    [∀ i, SelectableType (spec.range i)] :
+    spec →[QueryCache spec]ₛₒ unifSpec :=
+  (unifOracle ∘ₛₒ cachingOracle).maskState
+    (Equiv.prodPUnit (QueryCache spec))
