VCVio/OracleComp/SimSemantics/QueryTracking/CountingOracle.lean
@@ -18,6 +18,7 @@ open OracleComp
 
 namespace OracleSpec
 
+@[inline, reducible]
 def QueryCount (spec : OracleSpec) : Type := spec.ι → ℕ
 
 variable {spec : OracleSpec}
@@ -36,7 +37,7 @@ open OracleComp OracleSpec
 
 def countingOracle {spec : OracleSpec} :
     spec →[QueryCount spec]ₛₒ spec :=
-  λ i ⟨t, qc⟩ ↦ (·, qc.increment i 1) <$> query i t
+  λ i t qc ↦ (·, qc.increment i 1) <$> query i t
 
 -- def countingOracle {spec : OracleSpec} :
 --   spec →[List spec.ι]ₛₒ spec :=
