VCVio/OracleComp/SimSemantics/QueryTracking/LoggingOracle.lean
@@ -19,12 +19,18 @@ def QueryLog.logQuery {spec : OracleSpec} (log : QueryLog spec) {i : spec.ι}
     (t : spec.domain i) (u : spec.range i) : QueryLog spec :=
   Function.update log i ((t, u) :: log i)
 
+def QueryLog.wasQueried {spec : OracleSpec} (log : QueryLog spec)
+    (i : spec.ι) (t : spec.domain i) : Bool :=
+  match (log i).find? (λ (t', _) ↦ t = t') with
+  | Option.some _ => true
+  | Option.none => false
+
 end OracleSpec
 
 open OracleComp OracleSpec
 
 def loggingOracle {spec : OracleSpec} :
     spec →[QueryLog spec]ₛₒ spec :=
-  λ i ⟨t, log⟩ ↦ do
+  λ i t log ↦ do
     let u ← query i t
     return (u, log.logQuery t u)
