VCVio/OracleComp/SimSemantics/QueryTracking/SeededOracle.lean
@@ -4,11 +4,16 @@ Released under Apache 2.0 license as described in the file LICENSE.
 Authors: Devon Tuma
 -/
 import VCVio.OracleComp.SimSemantics.Simulate
+import VCVio.OracleComp.SimSemantics.QueryTracking.CountingOracle
+import VCVio.OracleComp.Constructions.Replicate
+import VCVio.OracleComp.Constructions.UniformSelect
 
 /-!
 # Seeding Results of Queries
 
 -/
+
+open OracleComp OracleSpec BigOperators
 
 variable {spec : OracleSpec}
 
@@ -17,13 +22,35 @@ namespace OracleSpec
 def QuerySeed (spec : OracleSpec) : Type :=
   (i : spec.ι) → List (spec.range i)
 
+namespace QuerySeed
+
+instance : Coe (QuerySeed spec) (QueryCount spec) where
+  coe := λ qs i ↦ (qs i).length
+
+def toCount (qs : QuerySeed spec) : QueryCount spec := λ i ↦ (qs i).length
+
 instance : EmptyCollection (QuerySeed spec) := ⟨λ _ ↦ []⟩
+
+def addValues (qs : QuerySeed spec) {i : spec.ι}
+    (us : List (spec.range i)) : QuerySeed spec :=
+  λ j ↦ qs j ++ if h : j = i then h ▸ us else ∅
+
+def takeAtIndex (qs : QuerySeed spec) {i : spec.ι}
+    (n : ℕ) : QuerySeed spec :=
+  λ j ↦ if j = i then (qs j).take n else qs j
+
+def append (qs qs' : QuerySeed spec) : QuerySeed spec :=
+  λ i ↦ qs i ++ qs' i
+
+end QuerySeed
 
 end OracleSpec
 
-open OracleComp OracleSpec
-
 def seededOracle : spec →[QuerySeed spec]ₛₒ spec :=
-  λ i ⟨t, seed⟩ ↦ match seed i with
+  λ i t seed ↦ match seed i with
     | u :: us => return (u, Function.update seed i us)
-    | [] => (·, seed) <$> query i t
+    | [] => (·, ∅) <$> query i t
+
+namespace seededOracle
+
+end seededOracle
